math_project/MathProject/prooftree/test.lean
@@ -1,1 +1,53 @@
 import MathProject.prooftree.prop
+open Formula
+
+def A := atom "A"
+def B := atom "B"
+
+-- open Provable
+theorem t1 : [A] ⊢ A := by
+  apply Provable.Axiom
+  trivial
+
+theorem t2 : [] ⊢ A ⇒ A := by
+  exact Provable.ImpIntro t1
+
+theorem t3 : [A, B] ⊢ A ∧ B := by
+  apply Provable.AndIntro
+  · apply Provable.Axiom
+    trivial
+  · apply Provable.Axiom
+    trivial
+
+theorem t4 : [] ⊢ A ⇒ B ⇒ A ∧ B := by
+  apply Provable.ImpIntro
+  apply Provable.ImpIntro
+  apply Provable.AndIntro
+  · apply Provable.Axiom
+    trivial
+  · apply Provable.Axiom
+    trivial
+
+def P1 : Option ProofState := Assume A
+#eval P1
+
+def P2 : Option ProofState := by
+  apply Imp_I A
+  exact (Assume A)
+#eval P2
+
+def P3 : Option ProofState := by
+  apply And_I
+  · exact Assume A
+  · exact Assume B
+#eval P3
+
+def P4 : Option ProofState := by
+  apply Imp_I A
+  apply Imp_I B
+  apply And_I
+  · exact Assume A
+  · exact Assume B
+#eval P4
+
+-- example : [A] ⊢ A := by
